TODO.md
@@ -5,8 +5,10 @@
         - Yes, because initial assignments are predicates of object, while formulas have atoms of term
         - PDDL_FORMULAS do not need a parameter
 - Implement conversion from ML types to Isabelle types
-    - [ ] Is there some existing function that converts strings to rational numbers?
-    - The assignment must be disambiguated after the function declarations have been parsed and proven well-formed.
+    - [x] Is there some existing function that converts strings to rational numbers?
+    - [ ] Prove conversion to rationals correct
+    - [ ] Implement a function to combine conditional effect lists
+    - [x]The assignment must be disambiguated after the function declarations have been parsed and proven well-formed.
         - This can be assumed, since the domain and problem declarations must habe been proven well-formed by the time action schemas are converted.
     - Domain declarations
     - Problem declarations
